---
aliases:
  - The equivalence theorem
tags:
  - logic
"References:": 
cssclasses: 
sr-due: 2024-06-06
sr-interval: 29
sr-ease: 290
---

## Propositional logic: 

> [!NOTE] Theorem:
> 
Let $F_A$ be the notation corresponding to a formula in Propositional calculus which includes the formula A. Then the equivalence theorem states:
>$$
>\text { If } \vdash \mathbf{A} \leftrightarrow \mathbf{B} \text 
>{then } \vdash \mathbf{F}_{\mathbf{A}} \leftrightarrow 
>\mathbf{F}_{\mathbf{B}}
>$$


+ $F_B$ is the formula we obtain when A is replaced by B in $F_A$
+ Namely: We can replace every A for a B and the formula is equivalent.

## Predicate logic: 

> [!NOTE] Theorem:
> The same stated above can also be aplied in predicate logic for both quantifiers.
> $$
> 
\begin{aligned}
& \text { Lemma 1: If } \vdash \mathbf{A}(\mathbf{y}) \leftrightarrow \mathbf{B}(\mathbf{y}) \\
& \text { then } \forall \mathbf{x} \mathbf{A}(\mathbf{x}) \leftrightarrow \forall \mathbf{x} \mathbf{B}(\mathbf{x})
\end{aligned}
>$$
>$$
>\begin{aligned}
& \text { Lemma 2: If } \vdash \mathbf{A}(\mathbf{y}) \leftrightarrow \mathbf{B}(\mathbf{y}) \\
& \text { then } \exists \mathbf{x} \mathbf{A}(\mathbf{x}) \leftrightarrow \exists \mathbf{x} \mathbf{B}(\mathbf{x})
\end{aligned}
>$$

